Interrupts: refactor

theories/prelude/interrupts.v
@@ -86,16 +86,20 @@ Proof. solve_inhabited. Qed.
 #[global] Instance InterruptSignal_eq_dec : EqDecision InterruptSignal.
 Proof. solve_decision. Defined.
 
-Definition int_types_match (sig : InterruptSignal) (ty : IntConfig) : Prop :=
+Definition int_trigger_match (sig : InterruptSignal) (trg : IntTrigger) : Prop :=
   match sig with
-  | LevelSig high => ty.(int_trigger) = TriggerLevel (negb high)
+  | LevelSig high => trg = TriggerLevel (negb high)
     (* ^ [high = true] is a valid level trigger only if
          [TriggerLevel false (*= active_low*)]. *)
-  | EdgeSig => ty.(int_trigger) = TriggerEdge
+  | EdgeSig => trg = TriggerEdge
   end.
+#[global] Instance int_trigger_match_dec sig trg : Decision (int_trigger_match sig trg).
+Proof. case: sig => /=; by apply: _. Defined.
 
+Definition int_types_match (sig : InterruptSignal) (ty : IntConfig) : Prop :=
+  int_trigger_match sig ty.(int_trigger).
 #[global] Instance int_types_match_decision sig cfg : Decision (int_types_match sig cfg).
-Proof. case: cfg => ?; case: sig => /=; by apply: _. Defined.
+Proof. case: cfg => ?; by apply: _. Defined.
 
 (** [intcfg_valid cfg own sig] means that [cfg] matches [sig], the interrupt line was
     configured [IntEnabled], and the owner is [own] (guest or host). *)
